examples/webmodel/OAuth.RP.fst
@@ -4,7 +4,7 @@
 module OAuth.RP
 
 open FStar.All
-open FStar.Heap
+open FStar.Ref
 open FStar.IO
 open Web.Origin
 open Web.URI
@@ -14,24 +14,28 @@ open Browser.Datatypes
 open AuxiliaryFunctions
 open Browser.StringFunctions
 open Browser.Model.Interface
-open NetworkRequestInterface
+open Network.Interface
 open OAuth.Datatypes
+
+#reset-options "--z3rlimit 100"
 
 (* ***** RP.COM ***** *)
 let rpurl = ({c_origin=rpori;c_uname=emptyString (SecretVal [rpori]);c_pwd=emptyString (SecretVal [rpori]);c_path=[];c_querystring=[];c_fragment=emptyString (SecretVal [rpori])})
 let rpuri = mk_uri rpurl
 
-val checkRPReq : req:request -> Tot (b:bool)
-let checkRPReq req =
-  match (Request?.rsl req) with
-  | PublicVal -> true
-  | SecretVal ol -> List.mem rpori ol
+(* data related to different ips - already present through registration *)
+val rpCD : (FStar.ST.ref clientData)
+let rpCD = ST.alloc [(ipori, clientIDRPIP, clientSecretRPIP)]
 
-val rpReqLemma : req:request -> Lemma (requires (checkRPReq req)) (ensures (restricts (Request?.rsl req) (SecretVal [rpori]))) [SMTPat (checkRPReq req)]
-let rpReqLemma req = ()
+val rpLS : (FStar.ST.ref loginSession)
+let rpLS = ST.alloc [] 
+
+val getRPClientID : torigin -> St (option (s:secretVal{Secret?.s s = PublicVal}))
+let getRPClientID t = getClientID (!rpCD) t  
 
 (* (\* use a browser for sending request containing authcode from RP to IP at the end of the protocol *\) *)
-let rpbr :ref browser = ST.alloc (init_browser) 
+(* val rpbr : (ref browser) *)
+(* let rpbr = ST.alloc (init_browser)  *)
 (* let irp = match (set_unique_id !rpb) with | (f, s) -> rpb := s; f (\* Get a unique_id (f) and browser (s) *\) *)
 (* let rpdoc = {dloc=rpuri;dref=blank_uri;dori=(mk_aorigin rpurl.c_origin);dHTTPS="none";drefPol=RP_OriginWhenCO;dCSP=[];dsbox=[];} *)
 (* (\* create a window in the browser to send the request with "rpdoc" as the document *\) *)
@@ -41,10 +45,10 @@ let rpbr :ref browser = ST.alloc (init_browser)
 (*       (rpb := ({(!rpb) with windows=newwin::(!rpb).windows})); newwin *)
 
 (* send the initial login request to the IP *)
-val rpLoginIPAuth : r:request -> ML (resp:actResponse{requestResponseValid r resp}) 
+val rpLoginIPAuth : r:browserRequest -> ML (resp:actResponse{requestResponseValid r resp}) 
 let rpLoginIPAuth r =
-  let urisl = s_getReqURISecLevel r in
-  let ruri = mk_uri (s_getRequestURI #urisl r) in (* get the request url *)
+  let urisl = (BRequest?.rsl r) in
+  let ruri = (firstElement (BRequest?.rf r).requrl) in (* get the request url *)
   let qs = getQS ruri in
   let ip = getQSVal #urisl qs "IP" in
   if s_equal #urisl #PublicVal ip "ip" then 
@@ -53,7 +57,7 @@ let rpLoginIPAuth r =
     let sid = (genSecret sl) in
     let state = (genSecret sl) in 
     match (getRPClientID ipori) with
-    | None -> (print_string ("Error: Client id not found\n" ); (defErrResponse))
+    | None -> (print_string ("Error: Client id not found\n" ); (defErrResponse rpori (BRequest?.rf r).reqb))
     | Some clid ->
     (
       let cid = declassify #PublicVal (getSecret clid) in 
@@ -61,16 +65,16 @@ let rpLoginIPAuth r =
       rpLS := List.append logsession (!rpLS));
       let respuri = ({c_origin=ipori;c_uname=emptyString sl;c_pwd=emptyString sl;c_path=[classify #PublicVal "authEP" sl];c_querystring=[(classify #PublicVal "client_id" sl,classify #PublicVal cid sl);(classify #PublicVal "redirect_uri" sl, classify #PublicVal "https://rp.com:443/codeEP/" sl);(classify #PublicVal "origin" sl, classify #PublicVal "https://rp.com:443/" sl);(classify #PublicVal "csrftoken" sl,getSecret state)];c_fragment=emptyString sl}) in
       let rpREP = curi_to_hstring respuri in 
-      let rpResp = ActResponse sl ({resptype="default";respcode=301;respurl=[]; resphead=[("Set-Cookie", (mk_svheaderval sid));("Location", (mk_headerval rpREP))]; respbody=(emptyString sl);resptrail=[];respHTTPS="modern";respCSP=cspPol;respCORS=[];resploc=None;respRedSec=sl}) in
+      let rpResp = ActResponse sl ({respori=rpori;respdest=(BRequest?.rf r).reqb;resptype="default";respcode=301;respurl=[]; resphead=[("Set-Cookie", (mk_svheaderval sid));("Location", (mk_headerval rpREP))]; respbody=(emptyString sl);resptrail=[];respHTTPS="modern";respCSP=cspPol;respCORS=[];resploc=None;respRedSec=sl}) in
       (rpResp)
       ))
-  else if s_equal #urisl #PublicVal ip "badip" then
+  else if s_equal #urisl #PublicVal ip "badip" then 
   (
     let sl = (SecretVal [rpori;badipori]) in
     let sid = (genSecret sl) in
     let state = (genSecret sl) in
     match (getRPClientID ipori) with (* getting ipori's client_id as the badip will replace it eventually *)
-    | None -> (print_string ("Error: Client id not found\n" ); (defErrResponse))
+    | None -> (print_string ("Error: Client id not found\n" ); (defErrResponse rpori (BRequest?.rf r).reqb))
     | Some clid ->
     (
       let cid = declassify #PublicVal (getSecret clid) in 
@@ -80,77 +84,77 @@ let rpLoginIPAuth r =
       let usl = (SecretVal [rpori;ipori]) in
       let respuri = ({c_origin=ipori;c_uname="";c_pwd="";c_path=["authEP"];c_querystring=[("client_id",cid);("redirect_uri","https://rp.com:443/codeEP/");("origin","https://rp.com/");("csrftoken",declassify #sl (getSecret state))];c_fragment=""}) in
       let rpREP = classify #PublicVal (curi_to_hstring respuri) usl in
-      let rpResp = ActResponse usl ({resptype="default";respcode=301;respurl=[]; resphead=[("Set-Cookie", (mk_headerval (classify #PublicVal (declassify #sl (getSecret sid)) usl)));("Location", (mk_headerval rpREP))]; respbody=(emptyString usl);resptrail=[];respHTTPS="modern";respCSP=cspPol;respCORS=[];resploc=None;respRedSec=usl}) in
+      let rpResp = ActResponse usl ({respori=rpori;respdest=(BRequest?.rf r).reqb;resptype="default";respcode=301;respurl=[]; resphead=[("Set-Cookie", (mk_headerval (classify #PublicVal (declassify #sl (getSecret sid)) usl)));("Location", (mk_headerval rpREP))]; respbody=(emptyString usl);resptrail=[];respHTTPS="modern";respCSP=cspPol;respCORS=[];resploc=None;respRedSec=usl}) in
       print_string ("IP is not ip.com:" ^ (curi_to_hstring respuri) ^ "\n" );
       (rpResp)
       ))
-  else (print_string ("IP is not ip.com:" ^ (declassify ip) ^ "\n" ); (defErrResponse))
+  else (print_string ("IP is not ip.com:" ^ (declassify ip) ^ "\n" ); (defErrResponse rpori (BRequest?.rf r).reqb))
 
-val getRPLoginIPAuth : r:request -> ML (ret:retReqResp{isValidRetResp r ret})
+
+val getRPLoginIPAuth : r:browserRequest -> ML (ret:retReqResp{isValidRetResp (BrowserRequest r) ret})
 let getRPLoginIPAuth r = (let resp = rpLoginIPAuth r in RetResponse resp)
 
+
 (* Compact authcode resend method for the RP *)
-val rpReqCodeEP : request -> browser -> cowindow ->  ML (option (r:request{notForbiddenHeaderfieldInReqHeader (Request?.rf r).reqhead}))
-let rpReqCodeEP r rpb rpsw =
-  let urisl = s_getReqURISecLevel r in
-  let ruri = mk_uri (s_getRequestURI #urisl r) in (* get the request url *)
+val rpReqCodeEP : browserRequest ->  ML (option (sr:serverRequest{notForbiddenHeaderfieldInReqHeader (SRequest?.srf sr).sreqhead}))
+let rpReqCodeEP r =
+  let urisl = (BRequest?.rsl r) in
+  let ruri = (firstElement (BRequest?.rf r).requrl) in (* get the request url *)
   let qs = getQS #urisl (ruri) in
   let csrftoken = mk_secretval (getQSVal #urisl qs "csrftoken") in
   let actualIP = mk_secretval (getQSVal #urisl qs "Issuer") in
   let ip = getIPLogin !rpLS csrftoken in (* determine the IP based on the state-token *)
-  if (ip = blank_origin) then 
+  if (ip = blank_origin) then
     (None)
-  else if ((declassify #urisl (getSecret actualIP)) = (origin_to_string ip)) then 
-    (print_string ("Actual IP: " ^ (declassify #urisl (getSecret actualIP)) ^ "\nMy IP: " ^ (origin_to_string ip));
+  else if ((declassify #urisl (getSecret actualIP)) = (origin_to_string ip)) then
+    (
     let urisl = SecretVal [ip] in
     let code = declassify (getQSVal #(URI?.usl ruri) qs "authcode") in
-    match (getRPClientID ip) with 
+    match (getRPClientID ip) with
     | None -> (print_string ("Error: Client id not found with req-code\n" ); None)
     | Some clid ->
-	let cid = declassify #PublicVal (getSecret clid) in 
+	let cid = declassify #PublicVal (getSecret clid) in
 	(match (getCDSecret (!rpCD) ip) with
 	| None -> (* get client data secret is none for the ip -- may be the client_secret was not established *)
 	   (
 	   (* The port is required to pass isOriginSec in StringFunctions *)
 	   let rturi = ({c_origin=ip;c_uname=emptyString urisl;c_pwd=emptyString urisl;c_path=[(classify #PublicVal "tokenEP" urisl)];c_querystring=[((classify #PublicVal "client_id" urisl), classify #PublicVal cid urisl);((classify #PublicVal "redirect_uri" urisl),(classify #PublicVal "https://rp.com:443/codeEP/" urisl));((classify #PublicVal "authcode" urisl),(classify #PublicVal code urisl))];c_fragment=emptyString urisl}) in
-	   let nreq = Request urisl ({reqm = "POST"; requrl = [(mk_uri rturi)]; reqhead = []; reqo = mk_aorigin ((URI?.u (CWindow?.cwloc rpsw)).c_origin); reqw = (Some rpsw); reqinit = ""; reqtype = ""; reqdest = ""; reqtarget = None; reqredirect = 0; reqredmode = "follow"; reqref = (Client rpsw); reqrefPolicy = RP_OriginWhenCO; reqnonce = ""; reqparser = ""; requnsafe = false; reqpreflight = false; reqsync = false; reqmode = NoCORS; reqtaint = "basic"; reqcredm = "omit"; reqcredflag = false; reqbody = (emptyString urisl); corsflag = false; corspfflag = false; authflag = false; recflag = false}) in
-	   let (r, req, tw, nb) = navigateWindow rpb rpsw rpsw (RequestResource nreq) "other" in
-	   rpbr := nb; (req)
+	   let nreq = SRequest urisl ({sreqm = "POST"; srequrl = [(mk_uri rturi)]; sreqhead = []; sreqo = rpori; sreqtype = ""; sreqnonce = ""; sreqmode = NoCORS; sreqbody = (emptyString urisl);}) in
+	   Some nreq
 	   )
 	| Some sec ->
 	   (
 	   secretOriginLemma ip (Secret?.s sec);
 	   let cs = classify #(Secret?.s sec) (getSecret #(Secret?.s sec) (sec)) urisl in
 	   let rturi = ({c_origin=ip;c_uname=emptyString urisl;c_pwd=emptyString urisl;c_path=[(classify #PublicVal "tokenEP" urisl)];c_querystring=[((classify #PublicVal "client_id" urisl), classify #PublicVal cid urisl);((classify #PublicVal "redirect_uri" urisl),(classify #PublicVal "https://rp.com:443/codeEP/" urisl));((classify #PublicVal "authcode" urisl),(classify #PublicVal code urisl));((classify #PublicVal "client_secret" urisl),cs)];c_fragment=emptyString urisl}) in
-	   let nreq = Request urisl ({reqm = "POST"; requrl = [(mk_uri rturi)]; reqhead = []; reqo = mk_aorigin ((URI?.u (CWindow?.cwloc rpsw)).c_origin); reqw = (Some rpsw); reqinit = ""; reqtype = ""; reqdest = ""; reqtarget = None; reqredirect = 0; reqredmode = "follow"; reqref = (Client rpsw); reqrefPolicy = RP_OriginWhenCO; reqnonce = ""; reqparser = ""; requnsafe = false; reqpreflight = false; reqsync = false; reqmode = NoCORS; reqtaint = "basic"; reqcredm = "omit"; reqcredflag = false; reqbody = (emptyString urisl); corsflag = false; corspfflag = false; authflag = false; recflag = false}) in
-	   let (r, req, tw, nb) = navigateWindow rpb rpsw rpsw (RequestResource nreq) "other" in
-	   rpbr := nb; (req)
+	   let nreq = SRequest urisl ({sreqm = "POST"; srequrl = [(mk_uri rturi)]; sreqhead = []; sreqo = rpori; sreqtype = ""; sreqnonce = ""; sreqmode = NoCORS; sreqbody = (emptyString urisl);}) in
+	   Some nreq
 	   )))
   else (print_string ("Error: The IP does not match\n"); None)
 
-val getRPReqCodeEP : r:request -> ML (ret:retReqResp{isValidRetResp r ret})
-let getRPReqCodeEP r = 
-  (* use a browser for sending request containing authcode from RP to IP at the end of the protocol *)
-  let rpb = (init_browser) in
-  let (irp, sb) = (set_unique_id rpb) in  (* Get a unique_id (f) and browser (s) *)
-  let rpdoc = ({dloc=rpuri;dref=blank_uri;dori=(mk_aorigin rpurl.c_origin);dHTTPS="none";drefPol=RP_OriginWhenCO;dCSP=[];dsbox=[];}) in
-   (* create a window in the browser to send the request with "rpdoc" as the document *)
-  let hist = (HistEntry (URI?.usl rpuri) (URI?.u rpuri) get_time rpdoc irp) in 
-  let newwin = (win_to_cowin ({winid=irp;wname="";wloc=rpuri;wframes=[];wopener=None;wparent=None;whist={hlhe=[hist];hcur=1};wdoc=(rpdoc);wsbox=[];})) in
-  (match rpReqCodeEP r ({(sb) with windows=newwin::(sb).windows}) newwin with | None -> RetResponse defErrResponse | Some req -> RetRequest req)
+
+val getRPReqCodeEP : r:browserRequest -> ML (ret:retReqResp{isValidRetResp (BrowserRequest r) ret})
+let getRPReqCodeEP r = (match rpReqCodeEP r with | None -> RetResponse (defErrResponse rpori (BRequest?.rf r).reqb) | Some req -> RetRequest (ServerRequest req))
+
 
 (* For different requests, return different responses *)
-val rpReqResp : r:request -> ML (ret:retReqResp{isValidRetResp r ret})
-let rpReqResp r =
-    let urisl = s_getReqURISecLevel r in
-    let ruri = mk_uri (s_getRequestURI #urisl r) in (* get the request url *)
-    if checkRPReq r && (getPort ruri) = (Some 443) then (* Only accept secure connections (HTTPS) *)
-    (
-    if (checkEP r "login-ipauth") then (* if the end-point is login with IP *)
-      (getRPLoginIPAuth r)
-    else if (checkEP r "codeEP") then (* auth-code end-point *)
-      (getRPReqCodeEP r)
-    else (RetResponse defErrResponse)
-    )
-    else (print_string ("IP is not ip.com:" ^ (declassify (curi_to_hstring (s_getRequestURI #urisl r))) ^ "\n" ); (RetResponse defErrResponse))
+val rpReqResp : req:anyRequest -> ML (ret:retReqResp{isValidRetResp req ret})
+let rpReqResp req =
+    match req with 
+    | BrowserRequest r ->
+	let urisl = (BRequest?.rsl r) in
+	let ruri = (firstElement (BRequest?.rf r).requrl) in (* get the request url *)
+	if (getPort ruri) = (Some 443) then (* Only accept secure connections (HTTPS) *)
+	(
+	if (checkEP r "login-ipauth") then (* if the end-point is login with IP *)
+	  (getRPLoginIPAuth r)
+	else if (checkEP r "codeEP") then (* auth-code end-point *)
+	  (getRPReqCodeEP r)
+	else (RetResponse (defErrResponse rpori (BRequest?.rf r).reqb))
+	)
+	else (print_string ("Insecure connection: \n" ); (* " ^ (declassify (curi_to_hstring (s_getRequestURI #urisl r))) ^ " *)
+	  (RetResponse (defErrResponse rpori (BRequest?.rf r).reqb)))
+    | ServerRequest r -> 
+	  (RetResponse (defErrResponse rpori (SRequest?.srf r).sreqo)) (* Impossible case*)
 
+  
